Launchbury/Cardinality-Domain-Lists.thy
@@ -1,4 +1,4 @@
-theory CallFutureCardinality
+theory "Cardinality-Domain-Lists"
 imports Vars "Nominal-HOLCF" Env "Cardinality-Domain" "Set-Cpo" "Env-Set-Cpo"
 begin
 
