Launchbury/CoCallImplTTree.thy
@@ -1,0 +1,20 @@
+theory CoCallImplTTree
+imports TTreeAnalysisSig "Env-Set-Cpo" CoCallAritySig "CoCallGraph-TTree"
+begin
+
+context CoCallArity
+begin
+  definition Fexp :: "exp \<Rightarrow> Arity \<rightarrow> var ftree"
+    where "Fexp e = (\<Lambda> a. ccTTree (edom (Aexp e \<cdot>a)) (ccExp e\<cdot>a))"
+  
+  lemma Fexp_simp: "Fexp e\<cdot>a = ccTTree (edom (Aexp e \<cdot>a)) (ccExp e\<cdot>a)"
+    unfolding Fexp_def
+    by simp
+
+  sublocale TTreeAnalysis Fexp.
+end
+
+
+
+end
+
