Launchbury/TTreeAnalysisSpec.thy
@@ -1,13 +1,13 @@
-theory FTreeAnalysisSpec
-imports FTreeAnalysisSig ArityAnalysisSpec CallFutureCardinality 
+theory TTreeAnalysisSpec
+imports TTreeAnalysisSig ArityAnalysisSpec "Cardinality-Domain-Lists"
 begin
 
 hide_const Multiset.single
 
-locale FTreeAnalysisCarrier = FTreeAnalysis + EdomArityAnalysis +
+locale TTreeAnalysisCarrier = TTreeAnalysis + EdomArityAnalysis +
   assumes carrier_Fexp: "carrier (Fexp e\<cdot>a) = edom (Aexp e\<cdot>a)"
 
-locale FTreeAnalysisCorrect = FTreeAnalysisCarrier +
+locale TTreeAnalysisCorrect = TTreeAnalysisCarrier +
   assumes Fexp_App: "many_calls x \<otimes>\<otimes> (Fexp e)\<cdot>(inc\<cdot>a) \<sqsubseteq> Fexp (App e x)\<cdot>a"
   assumes Fexp_Lam: "without y (Fexp e\<cdot>(pred\<cdot>n)) \<sqsubseteq> Fexp (Lam [y]. e) \<cdot> n"
   assumes Fexp_subst: "Fexp (e[y::=x])\<cdot>a \<sqsubseteq> many_calls x \<otimes>\<otimes> without y ((Fexp e)\<cdot>a)"
@@ -15,8 +15,8 @@ locale FTreeAnalysisCorrect = FTreeAnalysisCarrier +
   assumes Fun_repeatable: "isVal e \<Longrightarrow> repeatable (Fexp e\<cdot>0)"
   assumes Fexp_IfThenElse: "Fexp scrut\<cdot>0 \<otimes>\<otimes> (Fexp e1\<cdot>a \<oplus>\<oplus> Fexp e2\<cdot>a) \<sqsubseteq> Fexp (scrut ? e1 : e2)\<cdot>a"
 
-locale FTreeAnalysisCardinalityHeap = 
-  FTreeAnalysisCorrect + CorrectArityAnalysisLet + 
+locale TTreeAnalysisCardinalityHeap = 
+  TTreeAnalysisCorrect + CorrectArityAnalysisLet + 
   fixes Fheap :: "heap \<Rightarrow> exp \<Rightarrow> Arity \<rightarrow> var ftree"
   assumes carrier_Fheap: "carrier (Fheap \<Gamma> e\<cdot>a) = edom (Aheap \<Gamma> e\<cdot>a)"
   assumes Fheap_thunk: "x \<in> thunks \<Gamma> \<Longrightarrow> p \<in> paths (Fheap \<Gamma> e\<cdot>a) \<Longrightarrow> \<not> one_call_in_path x p \<Longrightarrow> (Aheap \<Gamma> e\<cdot>a) x = up\<cdot>0"
